chore: det of augmented system

chapter3.lean
@@ -87,6 +87,10 @@
 -- Untyped Booleans Language
 
 -- terms
+
+namespace myFirstType
+open myFirstType
+
 inductive t where
   | True : t
   | False : t
@@ -97,15 +101,36 @@ inductive tv : t → Prop where
   | True : tv t.True
   | False : tv t.False
 
--- evaluation, defined as an *inductive predicate*
-inductive t.EvaluatesTo : t → t → Prop
-  | EvaluatesToTrue: t.EvaluatesTo (.ite .True l r) l
-  | EvaluatesToFalse: t.EvaluatesTo (.ite .False l r) r
-  | EvaluatesToIf : (h : t.EvaluatesTo cd cd') → t.EvaluatesTo (.ite cd l r) (.ite cd' l r)
-
 #reduce sizeOf t.True -- 1
 #reduce sizeOf t.False -- 1
 #reduce sizeOf (t.ite t.True t.True t.False) -- 4
+
+-- evaluation, defined as an *inductive predicate*
+inductive t.EvaluatesTo : t → t → Prop
+  | EvaluatesToTrue {x l r} (hx : x = .ite .True l r) : t.EvaluatesTo x l
+  | EvaluatesToFalse {x l r} (hx : x = .ite .False l r) : t.EvaluatesTo x r
+  | EvaluatesToIf{x y l r cd cd' } (hx : x = .ite cd l r) (hy : y = .ite cd' l r) : (h : t.EvaluatesTo cd cd') → t.EvaluatesTo x y
+
+-- reduceCtorEq is an axiom in lean that, when creating an inductive type, none of the constructores are equal to each other.
+#check t.noConfusion
+theorem foo : t.True ≠ t.False := by
+  simp only [ne_eq, reduceCtorEq, not_false_eq_true]
+
+-- we first prove some inversion lemmas about what can (not) evaluate from what
+
+theorem TrueCantEvaluate (x : t): ¬ t.True.EvaluatesTo x := by
+  intro hcontra
+  cases hcontra
+  case EvaluatesToTrue r hx => simp only [reduceCtorEq] at hx
+  case EvaluatesToFalse l hx => simp only [reduceCtorEq] at hx
+  case EvaluatesToIf l r cd cd' h hx hy => simp only [reduceCtorEq] at hx
+
+theorem FalseCantEvaluate (x : t): ¬ t.False.EvaluatesTo x := by
+  intro hcontra
+  cases hcontra
+  case EvaluatesToTrue r hx => simp only [reduceCtorEq] at hx
+  case EvaluatesToFalse l hx => simp only [reduceCtorEq] at hx
+  case EvaluatesToIf l r cd cd' h hx hy => simp only [reduceCtorEq] at hx
 
 /-
   theorem 3.5.4: determinacy of one-step evaluation
@@ -113,28 +138,71 @@ inductive t.EvaluatesTo : t → t → Prop
   (note that '→' = 'EvaluatesTo')
 -/
 theorem OneStepDeterminacy (a b c : t) (hab : t.EvaluatesTo a b) (hac : t.EvaluatesTo a c) : b = c := by
-  revert c -- need to generalize c to be able to use it afterwards in the inductive cases
+  revert c
   induction hab
-  · case EvaluatesToTrue =>
-   intros c hac
-   cases hac
-   · case EvaluatesToTrue => rfl
-   · case EvaluatesToIf tthenc telsec =>
-      cases telsec -- absurd, t.True is a normal form, cannot EvaluatesTo.
-  · case EvaluatesToFalse =>
-      intros c hac
-      cases hac
-      · case EvaluatesToFalse => rfl
-      · case EvaluatesToIf tthen telse =>
-        cases telse -- absurd, t.False is a normal form, cannot EvaluatesTo.
-  · case EvaluatesToIf ac ac' al ar hacac' ih  =>
-      intros c thenRed
-      cases thenRed
-      · case EvaluatesToTrue => cases hacac' -- absurd, t.True is a normal form, cannot EvaluatesTo.
-      · case EvaluatesToFalse => cases hacac' -- absurd, t.False is a normal form, cannot EvaluatesTo.
-      · case EvaluatesToIf tthen telse =>
-          rw [ih]
-          exact telse
+  case EvaluatesToTrue x l r hx =>
+    intros c hac
+    cases hac
+    case EvaluatesToTrue r' hx' =>
+      subst hx
+      simp only [t.ite.injEq, true_and] at hx'
+      simp only [hx']
+    case EvaluatesToFalse l' hx' =>
+      -- contradiction:
+      -- hx : x = t.True.ite l r
+      -- hx' : x = t.False.ite l' c
+      subst hx
+      simp only [t.ite.injEq, reduceCtorEq, false_and] at hx'
+    case EvaluatesToIf l' r' cd cd' hcd hx' hc =>
+      subst hx
+      simp only [t.ite.injEq] at hx'
+      obtain ⟨h1, h2⟩ := hx'
+      subst h1
+      contradiction
+  case EvaluatesToFalse x l r hx =>
+    intros c hac
+    cases hac
+    case EvaluatesToTrue r' hx' =>
+      -- contradiction:
+      -- hx : x = t.True.ite l r
+      -- hx' : x = t.False.ite l' c
+      subst hx
+      simp only [t.ite.injEq, reduceCtorEq, false_and] at hx'
+    case EvaluatesToFalse l' hx' =>
+      subst hx
+      simp only [t.ite.injEq, true_and] at hx'
+      simp only [hx']
+    case EvaluatesToIf l' r' cd cd' hcd hx' hc =>
+      subst hx
+      simp only [t.ite.injEq] at hx'
+      obtain ⟨h1, h2⟩ := hx'
+      subst h1
+      contradiction
+  case EvaluatesToIf x y l r cd cd' hx hx' hy ih  =>
+    intros c hac
+    cases hac
+    case EvaluatesToTrue k hk =>
+      subst hk
+      simp at hx
+      obtain ⟨h1,h2,h3⟩ := hx
+      subst h1
+      contradiction
+    case EvaluatesToFalse k hk =>
+      subst hk
+      simp at hx
+      obtain ⟨h1,h2,h3⟩ := hx
+      subst h1
+      contradiction
+    case EvaluatesToIf lx rx cdx cd'x hcdx hcdx' hc =>
+      subst hx
+      simp only [t.ite.injEq] at hcdx'
+      obtain ⟨h1,h2,h3⟩ := hcdx'
+      subst h1
+      specialize ih cd'x hcdx
+      subst ih
+      subst hx' hc h2 h3
+      rfl
+
 
 /- def 8.
    a term t is in normal form if no evaluation rule applies to it
@@ -148,7 +216,16 @@ theorem ValueIsInNF (v : t) (h : tv v) : NormalForm v := by
   intro h' -- by contradiction, suppose ∃ tt such that v → tt
   obtain ⟨tt, htt⟩ := h'
   cases h -- by h, we know that v is eithet t.True or t.False, and no evaluation rule exists for these elements
-  <;> cases htt -- absurd
+  · case intro.True =>
+    cases htt
+    · case EvaluatesToTrue r hr => simp at hr
+    · case EvaluatesToFalse l hl => simp at hl
+    · case EvaluatesToIf l r cd cd' h hx hy => cases hx
+  · case intro.False =>
+    cases htt
+    · case EvaluatesToTrue r hr => simp at hr
+    · case EvaluatesToFalse l hl => simp at hl
+    · case EvaluatesToIf l r cd cd' h hx hy => cases hx
 
 /--
   Recall the principle of structural induction:
@@ -175,25 +252,25 @@ theorem NFImpValue (v : t) (h : NormalForm v) : tv v := by
       unfold NormalForm at h
       simp only [not_exists] at h
       specialize h l -- if ∀ (x : t), ¬(t.True.ite l r).EvaluatesTo x, then we can specialize with x = l: ¬(t.True.ite l r).EvaluatesTo l
-      have := t.EvaluatesTo.EvaluatesToTrue (r := r) (l := l) -- however, this rules exists!
+      have := t.EvaluatesTo.EvaluatesToTrue (r := r) (l := l) (x := t.True.ite l r) (by rfl) -- however, this rules exists!
       contradiction
     · -- same as above
       case False =>
       unfold NormalForm at h
       simp only [not_exists] at h
       specialize h r
-      have := t.EvaluatesTo.EvaluatesToFalse (r := r) (l := l)
+      have := t.EvaluatesTo.EvaluatesToFalse (r := r) (l := l) (x := t.False.ite l r) (by rfl)
       contradiction
     · -- v = ite cd l r, cd = ite cd' l' r', i.e., v = ite (ite cd' l' r') l r
       -- cd is not a value and by the inductive hp it is also not nf, i.e., ∃ tt' : cd → tt'
       -- however, if this is the case, then (v = ite cd l r) [EvaluatesToIf]→ (ite tt' l r) (this is the only viable rule!)
       -- and t is thus not nf either
       case ite cd' l' r' =>
-      have hIteNotTv' := IteNotTv (cd := cd') (l := l') (r := r')
-      simp only [NormalForm, not_exists, hIteNotTv', imp_false, Classical.not_forall,
+      have hIteNottv := IteNotTv (cd := cd') (l := l') (r := r')
+      simp only [NormalForm, not_exists, hIteNottv, imp_false, Classical.not_forall,
         Classical.not_not] at ihcd h
       obtain ⟨x, hx⟩ := ihcd
-      have := t.EvaluatesTo.EvaluatesToIf (cd := cd'.ite l' r') (cd' := x) (l := l) (r := r)
+      have := t.EvaluatesTo.EvaluatesToIf (cd := cd'.ite l' r') (cd' := x) (l := l) (r := r) (x := (cd'.ite l' r').ite l r ) (y := x.ite l r)
       simp_all only [imp_false, not_true_eq_false]
 
 /- 3.5.13: if we add a new rule things could go wild and the theorems might stop holding. -/
@@ -208,47 +285,51 @@ inductive t.FunnyEvaluatesTo : t → t → Prop
 theorem funnyEval₁ : (t.True.ite l r).FunnyEvaluatesTo l := t.FunnyEvaluatesTo.EvaluatesToTrue (l := l) (r := r)
 theorem funnyEval₂ : (t.True.ite l r).FunnyEvaluatesTo r := t.FunnyEvaluatesTo.EvaluatesToFunny (l := l) (r := r)
 
+end myFirstType
+
+namespace mySecondType
+
 /--  Untyped Booleans and Naturals: we introduce a new type t' which contains either elements from t (booleans) or natural numbers -/
 
-inductive t' where
-  | True : t'
-  | False : t'
-  | ite : t' → t' → t' → t'
-  | zero : t'
-  | succ : t' → t'
-  | pred : t' → t'
-  | iszero : t' → t'
+inductive t where
+  | True : t
+  | False : t
+  | ite : t → t → t → t
+  | zero : t
+  | succ : t → t
+  | pred : t → t
+  | iszero : t → t
   deriving Repr
 
-inductive tv' : t' → Prop where
-  | True : tv' t'.True
-  | False : tv' t'.False
+inductive tv : t → Prop where
+  | True : tv t.True
+  | False : tv t.False
 
-inductive nv' : t' → Prop where
-  | zero : nv' t'.zero
-  | succ n : nv' n → nv' (t'.succ n)
+inductive nv : t → Prop where
+  | zero : nv t.zero
+  | succ n : nv n → nv (t.succ n)
 
-inductive t'.EvaluatesTo : t' → t' → Prop
+inductive t.EvaluatesTo : t → t → Prop
 | -- ite true l r → l
-  EvaluatesToTrue {l r : t'} : t'.EvaluatesTo (True.ite l r) l
+  EvaluatesToTrue {l r : t} : t.EvaluatesTo (True.ite l r) l
 | -- ite false l r → r
-  EvaluatesToFalse {l r : t'} : t'.EvaluatesTo (False.ite l r) r
+  EvaluatesToFalse {l r : t} : t.EvaluatesTo (False.ite l r) r
 | -- (cd → cd') → (ite cd l r → ite cd' l r)
-  EvaluatesToIf (h : t'.EvaluatesTo cd cd') : t'.EvaluatesTo (cd.ite l r) (cd'.ite l r)
+  EvaluatesToIf (h : t.EvaluatesTo cd cd') : t.EvaluatesTo (t.ite cd l r) (t.ite cd' l r)
 | -- (v → v') → (succ v → succ v')
-  EvaluatesToSucc {v v' : t'} (h : EvaluatesTo v v') : (EvaluatesTo (t'.succ v) (t'.succ v'))
+  EvaluatesToSucc {v v' : t} (h : EvaluatesTo v v') : (EvaluatesTo (t.succ v) (t.succ v'))
 | -- pred 0 = 0
-  EvaluatesToZero : t'.EvaluatesTo (t'.pred t'.zero) (t'.zero)
+  EvaluatesToZero : t.EvaluatesTo (t.pred t.zero) (t.zero)
 | -- pred (succ nv) → nv
-  EvaluatesToPredSucc (h : nv' v) : t'.EvaluatesTo (t'.pred (t'.succ v))  (v)
+  EvaluatesToPredSucc (h : nv v) : t.EvaluatesTo (t.pred (t.succ v))  (v)
 | -- (v → v') → (pred v → pred v')
-  EvaluatesToPred (h : t'.EvaluatesTo v v') : t'.EvaluatesTo (t'.pred v) (t'.pred v')
+  EvaluatesToPred (h : t.EvaluatesTo v v') : t.EvaluatesTo (t.pred v) (t.pred v')
 | -- iszero 0 → true
-  EvaluatesToIsZeroZero : t'.EvaluatesTo (t'.iszero t'.zero) (t'.True)
+  EvaluatesToIsZeroZero : t.EvaluatesTo (t.iszero t.zero) (t.True)
 | -- iszero (succ nv) → false
-  EvaluatesToIsZeroSucc (h : nv' v) : t'.EvaluatesTo (t'.iszero (t'.succ v)) (t'.False)
-| -- (tt → tt') → (iszero tt → iszero tt')
-  EvaluatesToIsZero (h : t'.EvaluatesTo tt tt') : t'.EvaluatesTo (t'.iszero tt) (t'.iszero tt')
+  EvaluatesToIsZeroSucc (h : nv v) : t.EvaluatesTo (t.iszero (t.succ v)) (t.False)
+| -- (tt → tt) → (iszero tt → iszero tt)
+  EvaluatesToIsZero (h : t.EvaluatesTo tt tt') : t.EvaluatesTo (t.iszero tt) (t.iszero tt')
 
 /-- Excursus on inductive predicates and relations based on a set-theory-perspective,
   from https://link.springer.com/chapter/10.1007/3-540-61780-9_64
@@ -302,39 +383,39 @@ inductive t'.EvaluatesTo : t' → t' → Prop
 -/
 
 -- it is not true that given any t: True → t
-theorem NotTrueEvalTo (t : t') : ¬ t'.EvaluatesTo t'.True t := by
+theorem NotTrueEvalTo (v : t) : ¬ t.EvaluatesTo t.True v := by
   intro h -- suppose by hp. we have t'.EvaluatesTo t'.True t
   cases h -- then we evaluate the cases by which this hypothesi can be true: none!
 
 -- it is not true that given any t: False → t
-theorem NotFalseEvalTo (t : t') : ¬ t'.EvaluatesTo t'.False t := by
-  intro h -- suppose by hp. we have t'.EvaluatesTo t'.False t
+theorem NotFalseEvalTo (v : t) : ¬ t.EvaluatesTo t.False v := by
+  intro h -- suppose by hp. we have t.EvaluatesTo t.False t
   cases h -- then we evaluate the cases by which this hypothesi can be true: none!
 
 -- it is not true that given any t: zero → t
-theorem NotZeroEvalTo (t : t') : ¬ t'.EvaluatesTo t'.zero t := by
-  intro h -- suppose by hp. we have t'.EvaluatesTo t'.zero t
+theorem NotZeroEvalTo (v : t) : ¬ t.EvaluatesTo t.zero v := by
+  intro h -- suppose by hp. we have t.EvaluatesTo t.zero t
   cases h -- then we evaluate the cases by which this hypothesi can be true: none!
 
--- it is not true that a v : t' such that ∃ n : nv v can evaluate to a generic t
-theorem NotNvEvalTo (v t : t') (n : nv' v) : ¬ t'.EvaluatesTo v t := by
-  induction n generalizing t
+-- it is not true that a v : t such that ∃ n : nv v can evaluate to a generic t
+theorem NotNvEvalTo (v u : t) (n : nv v) : ¬ t.EvaluatesTo v u := by
+  induction n generalizing u
   · -- n = nv t'.zero, v' = t'.zero
-    case zero => exact NotZeroEvalTo t
-  · -- n = succ n' = nv (t'.succ n'), v' = t'.succ n'
-    -- with ihn : ∀ (t : t'), ¬v'.EvaluatesTo t
+    case zero => exact NotZeroEvalTo u
+  · -- n = succ n' = nv (t.succ n'), v' = t.succ n'
+    -- with ihn : ∀ (t : t), ¬v'.EvaluatesTo t
     -- and the goal will require to demonstrate ¬v'.succ.EvaluatesTo t
     case succ v' n ihn =>
-    intro h' -- suppose we can actually have an evaluation of (t'.succ v') → t
-    cases h' -- this can only happen by (t'.succ v')[EvaluatesToSucc]→ t
+    intro h' -- suppose we can actually have an evaluation of (t.succ v') → t
+    cases h' -- this can only happen by (t.succ v')[EvaluatesToSucc]→ t
     · case EvaluatesToSucc t₁' h =>
-      -- note that the rule says that given (h : EvaluatesTo t₁ t₁') then (EvaluatesTo (t'.succ t₁) (t'.succ t₁'))
-      -- we thus suppose there exists a t₁' such that v' → t₁', by which we conclude (t'.succ v') → (t'.succ t₁')
+      -- note that the rule says that given (h : EvaluatesTo t₁ t₁') then (EvaluatesTo (t.succ t₁) (t.succ t₁'))
+      -- we thus suppose there exists a t₁' such that v' → t₁', by which we conclude (t.succ v') → (t.succ t₁')
       -- we need to prove that the inductive hypothesis still holds: ¬ v' → (succ t₁')
       -- we apply the inductive hypothesis ¬v'.EvaluatesTo t with t = t₁' and given the evaluation in h.
       exact ihn t₁' h
 
-theorem OneStepDeterminacy' (a b c : t') (hab : t'.EvaluatesTo a b) (hac : t'.EvaluatesTo a c) : b = c := by
+theorem OneStepDeterminacy' (a b c : t) (hab : t.EvaluatesTo a b) (hac : t.EvaluatesTo a c) : b = c := by
   -- we use induction on the derivation rule hab
   induction hab generalizing c -- same as "revert c"
   · -- a [EvaluatesToTrue]→ b
@@ -386,7 +467,7 @@ theorem OneStepDeterminacy' (a b c : t') (hab : t'.EvaluatesTo a b) (hac : t'.Ev
       -- (cond₂ l r) = (cond' l r)
       case EvaluatesToIf cd'' hCdEvalToCd =>
       -- we exploit the congruence in functions and applications and construct
-      exact congrFun (congrFun (congrArg t'.ite (ihcond cd'' hCdEvalToCd)) l) r
+      exact congrFun (congrFun (congrArg t.ite (ihcond cd'' hCdEvalToCd)) l) r
   · -- a [EvaluatesToSucc]→ b
     -- i.e. a = succ v and hab : given (v → v') then (succ v) → (succ v')
     -- with a = succ v and b = succ v'
@@ -398,7 +479,7 @@ theorem OneStepDeterminacy' (a b c : t') (hab : t'.EvaluatesTo a b) (hac : t'.Ev
       -- and the goal b = c becomes:
       -- succ v' = succ v''
       case EvaluatesToSucc v'' hvEvalTov'' =>
-      exact congrArg t'.succ (ih v'' hvEvalTov'')
+      exact congrArg t.succ (ih v'' hvEvalTov'')
   · -- a [EvaluatesToZero]→ b
     -- i.e. a = zero
     case EvaluatesToZero =>
@@ -424,9 +505,9 @@ theorem OneStepDeterminacy' (a b c : t') (hab : t'.EvaluatesTo a b) (hac : t'.Ev
       case EvaluatesToPred v' hvEvalTov' =>
       -- we construct the numerical value of succ v
       -- using the constructors of nv, v and its numerical value
-      have hNv' : nv' (t'.succ v) := nv'.succ v hNv
+      have hnv : nv (t.succ v) := nv.succ v hNv
       -- and we exploit the fact that the numerical value can not be evaluated to anything
-      exact absurd hvEvalTov' (NotNvEvalTo _ _ hNv')
+      exact absurd hvEvalTov' (NotNvEvalTo _ _ hnv)
   · -- a [EvaluatesToPred] → b
     -- i.e. hab : a = pred v and hab : given (v → v') then (pred v) → (pred v')
     case EvaluatesToPred v v' hvEvalTov' ih =>
@@ -441,19 +522,19 @@ theorem OneStepDeterminacy' (a b c : t') (hab : t'.EvaluatesTo a b) (hac : t'.Ev
       -- which becomes succ c → v' in the hypotheses hab introduces
       -- the goal b = c becomes
       -- pred v' = c
-      case EvaluatesToPredSucc hNv'' =>
+      case EvaluatesToPredSucc hnv' =>
       -- we use the constructor of nv to
-      have hNv'' : nv' (t'.succ c) := nv'.succ c hNv''
+      have hnv' : nv (t.succ c) := nv.succ c hnv'
       -- no evaluation rule applies to numerical values, i.e., hvEvalTov' yields an absurd
-      -- given the construction of hNV''
-      exact absurd hvEvalTov' (NotNvEvalTo _ _ hNv'')
+      -- given the construction of hnv'
+      exact absurd hvEvalTov' (NotNvEvalTo _ _ hnv')
     · -- a [EvaluatesToPred]→ c
       -- i.e. hac : a = (pred v) and (pred v) → (pred v''),
       -- which relies on v → v''
       -- the goal b = c becomes
       -- pred v' = pred v'', we use the inductive hypothesis
       case EvaluatesToPred v'' hvEvalTov'' =>
-      exact congrArg t'.pred (ih v'' hvEvalTov'')
+      exact congrArg t.pred (ih v'' hvEvalTov'')
   · -- a [EvaluatesToIsZeroZero]→ b
     -- i.e. hab : (iszero zero) → True and thus a = iszero zero, b = True
     case EvaluatesToIsZeroZero =>
@@ -464,8 +545,8 @@ theorem OneStepDeterminacy' (a b c : t') (hab : t'.EvaluatesTo a b) (hac : t'.Ev
       -- however, a = iszero zero, and thus hac becomes:
       -- given zero → tt then iszero zero → iszero tt', which is absurd
       -- according to the inversion lemmas.
-      case EvaluatesToIsZero tt' hZeroEvalTott' =>
-      exact absurd hZeroEvalTott' (NotZeroEvalTo tt')
+      case EvaluatesToIsZero hZeroEvalTott' =>
+      exact absurd hZeroEvalTott' (NotZeroEvalTo _)
   · -- a [EvaluatesToIsZeroSucc]→ b
     -- i.e. given a v with numerical value nv v, then iszero (succ v) → false
     -- with a = iszero (succ v) and b = false
@@ -476,29 +557,29 @@ theorem OneStepDeterminacy' (a b c : t') (hab : t'.EvaluatesTo a b) (hac : t'.Ev
       -- i.e. hac : given (succ v) → v'' then (iszero (succ v)) → (iszero v'') remembering that a = iszero (succ v) from hab
       -- the goal b = c thus becomes
       -- false = iszero v''
-      case EvaluatesToIsZero v'' hvsuccEvalTov'' =>
+      case EvaluatesToIsZero  hvsuccEvalTov'' =>
       -- we construct the numerical value of succ v
-      have hNvSucc : nv' (t'.succ v) := nv'.succ v hNv
+      have hNvSucc : nv (t.succ v) := nv.succ v hNv
       -- and we show that the derivation (succ v) → v'' is absurd, since
       exact absurd hvsuccEvalTov'' (NotNvEvalTo _ _ hNvSucc)
   · -- a [EvaluatesToIsZero]→ b
     -- i.e. hab : given tt → tt' then (iszero tt) → (iszero tt')
     -- with a = iszero tt and b = iszero tt'
-    case EvaluatesToIsZero tt tt' httEvalTott' ih =>
+    case EvaluatesToIsZero tt httEvalTott' ih =>
     cases hac
     · -- a [EvaluatesToIsZeroZero]→ c
       -- i.e. hac : (iszero zero) → true however, a = iszero tt from hab,
       -- and if a = iszero zero in hab we would have zero → tt' in httEvalTott', which is absurd
       -- since zero can't evaluate to tt'
       case EvaluatesToIsZeroZero =>
-      exact absurd httEvalTott' (NotZeroEvalTo tt')
+      exact absurd httEvalTott' (NotZeroEvalTo _)
     · -- a [EvaluatesToIsZeroSucc]→ c
       -- i.e. hac : given a numerical value nv v, then (iszero (succ v)) → false
       -- with a = iszero (succ v). in hab, this would require iszero (succ v) → iszero tt'
       -- and in particular succ v → tt'
       case EvaluatesToIsZeroSucc v hNv =>
       -- we construct the numerical value for succ v
-      have hNvSucc : nv' (t'.succ v) := nv'.succ v hNv
+      have hNvSucc : nv (t.succ v) := nv.succ v hNv
       -- hypothesis httEvalTott' is absurd, since it supposes succ v → tt'
       exact absurd httEvalTott' (NotNvEvalTo _ _ hNvSucc)
     · -- a [EvaluatesToIsZero]→ c
@@ -507,177 +588,408 @@ theorem OneStepDeterminacy' (a b c : t') (hab : t'.EvaluatesTo a b) (hac : t'.Ev
       -- the goal b = c thus becomes
       -- iszero tt' = iszero tt'', we apply the inductive hypothesis
       case EvaluatesToIsZero tt'' httEvalTott' =>
-      exact congrArg t'.iszero (ih tt'' httEvalTott')
+      exact congrArg t.iszero (ih tt'' httEvalTott')
 
 /- def 3.5.9 a closed term is *stuck* if it is in normal form, but not a value -/
 
-def NormalForm' (tt : t') := ¬ ∃ tt', t'.EvaluatesTo tt tt'
+def NormalForm (tt : t) := ¬ ∃ tt', t.EvaluatesTo tt tt'
 
-def isStuck' (v : t') := (¬ nv' v) ∧ (¬ tv' v) ∧ NormalForm' v
+def isStuck (v : t) := (¬ nv v) ∧ (¬ tv v) ∧ NormalForm v
 
+end mySecondType
+
+namespace myThirdType
+
+open myThirdType
 
 /- 3.5.16: we enrich the semantics with a new term `wrong`, to formalize meaningless states and
   introduce rules that generate this term every time the semantics gets stuck. -/
 
-inductive t'' where
-  | True : t''
-  | False : t''
-  | ite : t'' → t'' → t'' → t''
-  | zero : t''
-  | succ : t'' → t''
-  | pred : t'' → t''
-  | iszero : t'' → t''
-  | wrong : t''
+inductive t where
+  | True : t
+  | False : t
+  | ite : t → t → t → t
+  | zero : t
+  | succ : t → t
+  | pred : t → t
+  | iszero : t → t
+  | wrong : t
   deriving Repr
 
 -- values
-inductive tv'' : t'' → Prop where
-  | True : tv'' t''.True
-  | False : tv'' t''.False
+inductive tv : t → Prop where
+  | True : tv t.True
+  | False : tv t.False
 
-inductive nv'' : t'' → Prop where
-  | zero : nv'' (t''.zero)
-  | succ n : nv'' n → nv'' (t''.succ n)
+inductive nv : t → Prop where
+  | zero : nv (t.zero)
+  | succ n : nv n → nv (t.succ n)
 
-inductive badNat : t'' → Prop where
-  | wrong : badNat t''.wrong
-  | badTrue : badNat t''.True
-  | badFalse : badNat t''.False
+inductive badNat : t → Prop where
+  | wrong : badNat t.wrong
+  | badTv : tv x → badNat x
 
-inductive badBool : t'' →  Prop  where
-  | wrong : badBool t''.wrong
-  | badBoolZero : badBool t''.zero
-  | badBoolNv n : badBool n → badBool (t''.succ n)
+inductive badBool : t →  Prop  where
+  | wrong : badBool t.wrong
+  -- | badBoolZero : badBool t.zero
+  -- | badBoolNvSucc n : badBool n → badBool (t.succ n) note that this allows succ wrong!
+  | badNv : nv x → badBool x
 
-inductive t''.AugmentedEvaluatesTo : t'' → t'' → Prop
+inductive t.AugmentedEvaluatesTo : t → t → Prop
 | -- ite true l r → l
-  EvaluatesToTrue {l r : t''} : t''.AugmentedEvaluatesTo (True.ite l r) l
+  EvaluatesToTrue {l r : t} : t.AugmentedEvaluatesTo (True.ite l r) l
 | -- ite false l r → r
-  EvaluatesToFalse {l r : t''} : t''.AugmentedEvaluatesTo (False.ite l r) r
+  EvaluatesToFalse {l r : t} : t.AugmentedEvaluatesTo (False.ite l r) r
 | -- (cd → cd') → (ite cd l r → ite cd' l r)
-  EvaluatesToIf (h : t''.AugmentedEvaluatesTo cd cd') : t''.AugmentedEvaluatesTo (cd.ite l r) (cd'.ite l r)
+  EvaluatesToIf (h : t.AugmentedEvaluatesTo cd cd')  : t.AugmentedEvaluatesTo (cd.ite l r) (cd'.ite l r)
 | -- (v → v') → (succ v → succ v')
-  EvaluatesToSucc {v v' : t''} (h : AugmentedEvaluatesTo v v') : (AugmentedEvaluatesTo (t''.succ v) (t''.succ v'))
+  EvaluatesToSucc {v v' : t} (h : AugmentedEvaluatesTo v v') : (AugmentedEvaluatesTo (t.succ v) (t.succ v'))
 | -- pred 0 = 0
-  EvaluatesToZero : t''.AugmentedEvaluatesTo (t''.pred t''.zero) (t''.zero)
+  EvaluatesToZero : t.AugmentedEvaluatesTo (t.pred t.zero) (t.zero)
 | -- pred (succ nv) → nv
-  EvaluatesToPredSucc (h : nv'' v) : t''.AugmentedEvaluatesTo (t''.pred (t''.succ v))  (v)
+  EvaluatesToPredSucc (h : nv v) : t.AugmentedEvaluatesTo (t.pred (t.succ v))  (v)
 | -- (v → v') → (pred v → pred v')
-  EvaluatesToPred (h : t''.AugmentedEvaluatesTo v v') : t''.AugmentedEvaluatesTo (t''.pred v) (t''.pred v')
+  EvaluatesToPred (h : t.AugmentedEvaluatesTo v v') : t.AugmentedEvaluatesTo (t.pred v) (t.pred v')
 | -- iszero 0 → true
-  EvaluatesToIsZeroZero : t''.AugmentedEvaluatesTo (t''.iszero t''.zero) (t''.True)
+  EvaluatesToIsZeroZero : t.AugmentedEvaluatesTo (t.iszero t.zero) (t.True)
 | -- iszero (succ nv) → false
-  EvaluatesToIsZeroSucc (h : nv'' v) : t''.AugmentedEvaluatesTo (t''.iszero (t''.succ v)) (t''.False)
+  EvaluatesToIsZeroSucc (h : nv v) : t.AugmentedEvaluatesTo (t.iszero (t.succ v)) (t.False)
 | -- (tt → tt') → (iszero tt → iszero tt')
-  EvaluatesToIsZero (h : t''.AugmentedEvaluatesTo tt tt') : t''.AugmentedEvaluatesTo (t''.iszero tt) (t''.iszero tt')
+  EvaluatesToIsZero (h : t.AugmentedEvaluatesTo tt tt') : t.AugmentedEvaluatesTo (t.iszero tt) (t.iszero tt')
 |-- ite badBool l r → wrong
-  EvaluatesToIfWrong (h : badBool cd) : t''.AugmentedEvaluatesTo (cd.ite l r) t''.wrong
+  EvaluatesToIfWrong (h : badBool cd) : t.AugmentedEvaluatesTo (cd.ite l r) t.wrong
 | -- succ badNat → wrong
-  EvaluatesToSuccWrong (h : badNat tt) : t''.AugmentedEvaluatesTo (succ tt) t''.wrong
+  EvaluatesToSuccWrong (h : badNat tt) : t.AugmentedEvaluatesTo (succ tt) t.wrong
 | -- pred badNat → wrong
-  EvaluatesToPredWrong (h : badNat tt) : t''.AugmentedEvaluatesTo (pred tt) t''.wrong
+  EvaluatesToPredWrong (h : badNat tt) : t.AugmentedEvaluatesTo (pred tt) t.wrong
 | -- iszero badNat → wrong
-  EvaluatesToIsZeroWrong (h : badNat tt) : t''.AugmentedEvaluatesTo (t''.iszero tt) t''.wrong
+  EvaluatesToIsZeroWrong (h : badNat tt) : t.AugmentedEvaluatesTo (t.iszero tt) t.wrong
 
-/-- Given that we can't mix different types in the same theorem, we first define a mapping from t' to t'' -/
-def map (e : t') : t'' :=
+/-- Given that we can't mix different types in the same theorem, we first define a mapping from mySecondType.t to t -/
+def map (e : mySecondType.t) : t :=
   match e with
-  | t'.True => t''.True
-  | t'.False => t''.False
-  | t'.ite cnd lhs rhs => t''.ite (map cnd) (map lhs) (map rhs)
-  | t'.zero => t''.zero
-  | t'.pred n => t''.pred (map n)
-  | t'.succ n => t''.succ (map n)
-  | t'.iszero n => t''.iszero (map n)
+  | .True => t.True
+  | .False => t.False
+  | .ite cnd lhs rhs => t.ite (map cnd) (map lhs) (map rhs)
+  | .zero => t.zero
+  | .pred n => t.pred (map n)
+  | .succ n => t.succ (map n)
+  | .iszero n => t.iszero (map n)
 
-@[simp]
-def ElimOftvTrue {C : Sort u} (h : ¬ tv' t'.True) : C := by
-  have : tv' t'.True := by constructor
-  contradiction
+-- badnat has two constructors: wrong and tv, we say that neither of these is legal
+theorem nvCantBeABadNatWrong (u : t) : nv u → ¬ u = t.wrong := by
+  intro h
+  induction h
+  · case zero => simp
+  · case succ ti iht ihti => simp
 
-@[simp]
-def ElimOftvFalse {C : Sort u} (h : ¬ tv' t'.False) : C := by
-  have : tv' t'.False := by constructor
-  contradiction
+theorem nvCantBeTv (u : t) : nv u→ ¬ tv u := by
+  intro h
+  induction h
+  · case zero => intro h; cases h
+  · case succ ti iht ihti => intro h; cases h
 
-@[simp]
-def ElimOfnvZero {C : Sort u} (h : ¬ nv' t'.zero) : C := by
-  have : nv' t'.zero := by constructor
-  contradiction
+theorem tvCantBeNv (u : t) : tv u→ ¬ nv u := by
+  intro h
+  induction h
+  · case True => intro h; cases h
+  · case False => intro h; cases h
+
+theorem nvCantBeABadNat (u : t) : nv u → ¬ badNat u := by
+  intro h hcontra
+  induction hcontra
+  · case wrong =>
+      have := nvCantBeABadNatWrong _ h
+      contradiction
+  · case badTv bad hbad =>
+      have := nvCantBeTv _ h
+      contradiction
+
+theorem tvCantBeABadBoolWrong (u : t) : tv u → ¬ u = t.wrong := by
+  intro h
+  induction h
+  · case True => simp
+  · case False => simp
+
+theorem tvCantBeABadBool (u : t) : tv u → ¬ badBool u := by
+  intro h hcontra
+  induction hcontra
+  · case wrong =>
+      have := tvCantBeABadBoolWrong _ h
+      contradiction
+  · case badNv bad hbad =>
+      have := tvCantBeNv _ h
+      contradiction
 
 -- it is not true that given any t: wrong → t
-theorem NotWrongEvalTo (t : t'') : ¬ t''.AugmentedEvaluatesTo t''.wrong t := by
-  intro h -- suppose by hp. we have t''.AugmentedEvaluatesTo t''.wrong t
+theorem NotWrongEvalTo (u : t) : ¬ t.AugmentedEvaluatesTo t.wrong u := by
+  intro h -- suppose by hp. we have t.AugmentedEvaluatesTo t.wrong t
   cases h -- then we evaluate the cases by which this hypothesis can be true: none!
 
-/-- We first prove the one-step determinacy of AugmentedEvaluatesTo, which will be useful to prove the subsequent lemma -/
-theorem OneStepDeterminacyAugmented (a b c : t'') (hab : t''.AugmentedEvaluatesTo a b) (hac : t''.AugmentedEvaluatesTo a c) : b = c := by
+-- todo: if nv' x then x can't evaluate to anything
+theorem NotnvEvalTo (u v : t) (h : nv v): ¬ t.AugmentedEvaluatesTo v u := by
+  induction h generalizing u
+  · case zero => intros h; cases h
+  · case succ ti vi ihn =>
+    intros hcontra
+    cases hcontra
+    · case EvaluatesToSucc vii ihvii => specialize ihn vii; contradiction
+    · case EvaluatesToSuccWrong vii =>
+      have := nvCantBeABadNat _ vi vii
+      exact this
+
+theorem NotBadBoolEvalTo (u v : t) (h : badBool v) : ¬ t.AugmentedEvaluatesTo v u := by
+  induction h
+  · case wrong => exact NotWrongEvalTo u
+  · case badNv nv hnv => exact NotnvEvalTo u nv hnv
+
+theorem nvEvalToNv (u v : t) (h₁ : nv u) (h₂ : tv v) : ¬ t.AugmentedEvaluatesTo u v := by
+  induction h₁
+  · case zero =>
+    intro hcontra
+    cases hcontra
+  · case succ n hn hn' =>
+    intro hcontra
+    cases hcontra
+    · case EvaluatesToSucc m hm =>
+      cases h₂
+    · case EvaluatesToSuccWrong hbad =>
+      have := nvCantBeABadNat n hn
+      contradiction
+
+theorem selfCantEvalToSelf (u : t) : ¬ t.AugmentedEvaluatesTo u u := by
+  apply Classical.byContradiction
+  intro hcontra
+  simp at hcontra
+  induction u
+  · case True => cases hcontra
+  · case False => cases hcontra
+  · case ite cd l r cd' ihl ihr =>
+    cases hcontra
+    · case EvaluatesToIf hif => exact cd' hif
+  · case zero => cases hcontra
+  · case succ s hs =>
+    cases hcontra
+    · case EvaluatesToSucc ihs => exact hs ihs
+  · case pred p hp =>
+    cases hcontra
+    · case EvaluatesToPred ihp => exact hp ihp
+  · case iszero z hz =>
+    cases hcontra
+    · case EvaluatesToIsZero ih => exact hz ih
+  · case wrong => cases hcontra
+
+theorem selfCantEvalToSucc (u v : t) (hnv : nv u) (huv : v = u.succ) (h : t.AugmentedEvaluatesTo u v) :
+    ¬ t.AugmentedEvaluatesTo u u.succ := by
+  induction h
+  <;> cases huv
+  · case EvaluatesToSucc.refl s p ih =>
+    exact NotnvEvalTo s.succ.succ s.succ hnv
+
+theorem nvOfEvalTonv (u v : t) (hnv : nv u) (heval : u.AugmentedEvaluatesTo v) : nv v := by
+  induction hnv generalizing v
+  · case zero =>
+    cases heval
+  · case succ s hs ih =>
+    cases heval
+    · case EvaluatesToSucc p hp =>
+      exact nv.succ p (ih p hp)
+    · case EvaluatesToSuccWrong hbad =>
+      have := nvCantBeABadNat s hs
+      contradiction
+
+-- becuse the semantics are cakk-by-value, the type systems are deterministic
+
+/-- We first prove the one-step determinacy of AugmentsedEvaluatesTo, which will be useful to prove the subsequent lemma -/
+theorem OneStepDeterminacyAugmented (a b c : t) (hab : t.AugmentedEvaluatesTo a b) (hac : t.AugmentedEvaluatesTo a c) : b = c := by
   induction hab generalizing c
   · case EvaluatesToTrue lhs rhs =>
     cases hac
     · case EvaluatesToTrue => rfl
     · case EvaluatesToIf lhs' ihl' => cases ihl'
-    · case EvaluatesToIfWrong hbad => cases hbad -- True is not a badBool!
+    · case EvaluatesToIfWrong hbad =>
+      -- True is not a badBool!
+      contradiction
   · case EvaluatesToFalse lhs rhs =>
     cases hac
     · case EvaluatesToFalse => rfl
     · case EvaluatesToIf lhs' ihl' => cases ihl'
-    · case EvaluatesToIfWrong hbad => cases hbad -- False is not a badBool!
+    · case EvaluatesToIfWrong hbad =>
+      -- False is not a badBool!
+      contradiction
   · -- a [EvaluatesToIf]→ b
+    -- a = cd.ite l r
+    -- b = cd'.ite l r
+    -- and ∃ h : cd.evalTo cd'
     case EvaluatesToIf cond cond' lhs rhs ihl ihr =>
     cases hac
     · case EvaluatesToTrue => cases ihl -- True does not evaluate to anything
     · case EvaluatesToFalse => cases ihl -- False does not evaluate to anything
     · case EvaluatesToIf cond'' ihc' =>
       specialize ihr cond''
-      exact congrFun (congrFun (congrArg t''.ite (ihr ihc')) lhs) rhs
+      exact congrFun (congrFun (congrArg t.ite (ihr ihc')) lhs) rhs
     · -- a [EvaluatesToIfWrong]→ c
       case EvaluatesToIfWrong hbad =>
       -- we want to show that if a = wrong then a [EvaluatesToIf]→ b is a contradiction
-      cases hbad
+      induction hbad generalizing cond'
       · case wrong => cases ihl
-      · case badBoolZero => cases ihl
-      · case badBoolNv bad hbad =>
+      · case badNv nvbad hbad =>
+        -- nvbad can't evaluate to cond'
+        have := NotnvEvalTo cond' nvbad hbad
+        contradiction
+  · -- a [EvaluatesToSucc]→ b
+    -- a = succ n
+    -- b = succ m
+    -- under the hypothesis that n [EvaluatesTo]→ m
+    case EvaluatesToSucc s r ihs ihr =>
+    cases hac
+    · -- hab and hac evaluate with the same rule
+      case EvaluatesToSucc r' h =>
+      specialize ihr r' h
+      simp [ihr]
+    · case EvaluatesToSuccWrong hbad =>
+      cases hbad
+      · case wrong => cases ihs
+      · case badTv htv =>
+        -- given htv, s can't evaluate to anything whose "succ" is different than wrong
+        cases htv
+        · case True => cases ihs
+        · case False => cases ihs
+  · case EvaluatesToZero =>
+    cases hac
+    · case EvaluatesToZero => rfl
+    · case EvaluatesToPred n hzero => cases hzero
+    · case EvaluatesToPredWrong hbad =>
+      -- zero is not badNat
+      have hnv : nv t.zero := nv.zero
+      have := nvCantBeABadNat t.zero hnv
+      contradiction
+  · case EvaluatesToPredSucc s ihs =>
+    cases hac
+    · case EvaluatesToPredSucc =>
+      rfl
+    · case EvaluatesToPred x hx =>
+      have := NotnvEvalTo x (s.succ) (by  constructor; apply ihs)
+      contradiction
+    · case EvaluatesToPredWrong badNat =>
+        -- NV can't be a badNat
+        have := nv.succ s ihs
+        have := nvCantBeABadNat s.succ this
+        contradiction
+  · case EvaluatesToPred s r ihs ihr =>
+    cases hac
+    · case EvaluatesToZero => cases ihs -- zero does not evaluate to anything
+    · case EvaluatesToPredSucc hnv =>
+      have := NotnvEvalTo r (c.succ) (by  constructor; apply hnv)
+      contradiction
+    · case EvaluatesToPred p hp =>
+      specialize ihr p hp
+      simp [ihr]
+    · case EvaluatesToPredWrong hbad =>
+      cases hbad
+      · case wrong => cases ihs
+      · case badTv h =>
+        have := tvCantBeNv s h
+        -- tv can't evalute to anything
+        cases h
+        · cases ihs
+        · cases ihs
+  · case EvaluatesToIsZeroZero =>
+    cases hac
+    · case EvaluatesToIsZeroZero => rfl
+    · case EvaluatesToIsZero v h => cases h
+    · case EvaluatesToIsZeroWrong hbad =>
+      have := nvCantBeABadNat t.zero nv.zero
+      contradiction
+  · case EvaluatesToIsZeroSucc s ihs =>
+      cases hac
+      · case EvaluatesToIsZeroSucc h => rfl
+      · case EvaluatesToIsZero v h =>
+        have ihs' := nv.succ s ihs
+        have := NotnvEvalTo v s.succ ihs'
+        contradiction
+      · case EvaluatesToIsZeroWrong h =>
+        have := nvCantBeABadNat s.succ (nv.succ s ihs)
+        contradiction
+  · case EvaluatesToIsZero s r ihsr ih =>
+      cases hac
+      · case EvaluatesToIsZeroZero => cases ihsr
+      · case EvaluatesToIsZeroSucc v ih =>
+        rename_i ihv
+        have := NotnvEvalTo r v.succ (nv.succ v ihv)
+        contradiction
+      · case EvaluatesToIsZero v h =>
+        simp only [t.iszero.injEq]
+        apply ih
+        exact h
+      · case EvaluatesToIsZeroWrong hbad =>
         cases hbad
-        · case wrong =>
-          cases ihl
-          · case EvaluatesToSucc h h' => cases h'
-          · case EvaluatesToSuccWrong h' =>
-            specialize ihr (t''.wrong.ite lhs rhs)
-            apply Eq.symm
+        · case wrong => cases ihsr
+        · case badTv htv =>
+          cases htv
+          · case True => cases ihsr
+          · case False => cases ihsr
+  · case EvaluatesToIfWrong cd l' r' hbad =>
+    cases hac
+    · case EvaluatesToTrue =>
+      have := tvCantBeABadBool (u := t.True) tv.True
+      contradiction
+    · case EvaluatesToFalse =>
+      have := tvCantBeABadBool (u := t.False) tv.False
+      contradiction
+    · case EvaluatesToIf cd' ih =>
+      cases hbad
+      · case wrong => cases ih
+      · case badNv hbad =>
+        have := NotnvEvalTo cd' cd hbad
+        contradiction
+    · case EvaluatesToIfWrong => rfl
+  · case EvaluatesToSuccWrong s ihs =>
+    cases hac
+    · case EvaluatesToSucc v ih =>
+      cases ihs
+      · case wrong => cases ih
+      · case badTv hv =>
+        cases hv
+        · case True => cases ih
+        · case False => cases ih
+    · case EvaluatesToSuccWrong => rfl
+  · case EvaluatesToPredWrong s ihs =>
+    cases hac
+    · case EvaluatesToZero =>
+      have := nvCantBeABadNat t.zero (nv.zero)
+      contradiction
+    · case EvaluatesToPredSucc h =>
+      have := nvCantBeABadNat c.succ (nv.succ c h)
+      contradiction
+    · case EvaluatesToPred v' hv' =>
+      cases ihs
+      · case wrong => cases hv'
+      · case badTv htv =>
+        cases htv
+        · case True => cases hv'
+        · case False => cases hv'
+    · case EvaluatesToPredWrong => rfl
+  · case EvaluatesToIsZeroWrong s ihs =>
+    cases hac
+    · case EvaluatesToIsZeroZero =>
+      have := nvCantBeABadNat t.zero nv.zero
+      contradiction
+    · case EvaluatesToIsZeroSucc u hu =>
+      have := nvCantBeABadNat u.succ (nv.succ u hu)
+      contradiction
+    · case EvaluatesToIsZero u hu =>
+      cases ihs
+      · case wrong => cases hu
+      · case badTv htv =>
+        cases htv
+        · case True => cases hu
+        · case False => cases hu
+    · case EvaluatesToIsZeroWrong => rfl
 
-            sorry
-        · case badBoolZero =>
-          cases ihl
-          · case EvaluatesToSucc h h' => cases h'
-          · case EvaluatesToSuccWrong h' =>
-            specialize ihr (t''.wrong.ite lhs rhs)
-            apply Eq.symm
-            apply ihr
-            sorry
-        · case badBoolNv =>
-          cases ihl
-          · case EvaluatesToSucc h h' => sorry
-          · case EvaluatesToSuccWrong h' =>
-            specialize ihr (t''.wrong.ite lhs rhs)
-            apply Eq.symm
-            apply ihr
-            sorry
-  · case EvaluatesToSucc s r ihs ihr => sorry
-  · case EvaluatesToZero => sorry
-  · case EvaluatesToPredSucc s ihs => sorry
-  · case EvaluatesToPred s r ihs ihr => sorry
-  · case EvaluatesToIsZeroZero => sorry
-  · case EvaluatesToIsZeroSucc s ihs => sorry
-  · case EvaluatesToIsZero s ihs r ihr => sorry
-  · case EvaluatesToIfWrong s ihs r ihs => sorry
-  · case EvaluatesToSuccWrong s ihs => sorry
-  · case EvaluatesToPredWrong s ihs => sorry
-  · case EvaluatesToIsZeroWrong s ihs => sorry
-
-/-- Then we prove that the augmented evaluations in t'' correspond to the def. of `stuck` in t' -/
-theorem stuck_iff (g : t'):
-    ((t''.AugmentedEvaluatesTo (map g) (t''.wrong))) ↔ (isStuck' g) := by
+/-- Then we prove that the augmented evaluations in t correspond to the def. of `stuck` in t' -/
+theorem stuck_iff (g : mySecondType.t):
+    ((t.AugmentedEvaluatesTo (map g) (t.wrong))) ↔ (mySecondType.isStuck g) := by
   induction g
   · case True =>
     simp [map]
@@ -740,7 +1052,7 @@ theorem stuck_iff (g : t'):
             exists lhs
           simp at this
           simp [map] at haug
-          have hexistsaug : t''.AugmentedEvaluatesTo (t''.ite t''.True (map lhs) (map rhs)) (map lhs) := t''.AugmentedEvaluatesTo.EvaluatesToTrue
+          have hexistsaug : t.AugmentedEvaluatesTo (t.ite t.True (map lhs) (map rhs)) (map lhs) := t.AugmentedEvaluatesTo.EvaluatesToTrue
           cases lhs <;> cases rhs
           · simp [map] at haug hexistsaug
             simp [this]
